FOL/Classical.lean
@@ -1,0 +1,4 @@
+import FOL.FOL
+
+def doubleNegAxiom (A : Formula) : Formula := .impl (neg (neg A)) A
+def excludedMiddleAxiom (A : Formula) : Formula := .or A (neg A)
