FOL/Tactics.lean
@@ -5,7 +5,10 @@ open Lean Meta Elab Tactic
 partial def getAllPositions (f : Formula) : List Pos :=
   match f with
   | .impl f1 f2 => .root :: (getAllPositions f1).map .left ++ (getAllPositions f2).map .right
+  | .and f1 f2 => .root :: (getAllPositions f1).map .left ++ (getAllPositions f2).map .right
+  | .or f1 f2 => .root :: (getAllPositions f1).map .left ++ (getAllPositions f2).map .right
   | .forall f1 => .root :: (getAllPositions f1).map .body
+  | .ex f1 => .root :: (getAllPositions f1).map .body
   | _ => [.root]
 
 -- A tactic to close the goal `Γ ⊢ f` if `f ∈ Γ`.
@@ -30,6 +33,20 @@ elab "derive_hyp" : tactic => do
 -- It tries to close the goal `Γ ⊢ f'` by finding `f ∈ Γ`, a position `p`, and a `LocalRule`
 -- such that `f` rewrites to `f'`.
 
-elab "derive_rewrite" : tactic => do
-  -- Not implemented yet, just a placeholder
-  pure ()
+syntax "derive_rewrite " term " at " term : tactic
+
+macro_rules
+  | `(tactic| derive_rewrite $rule at $pos) => `(tactic| apply Derives.rewrite_at $pos <;> exact $rule)
+
+-- Tactic to automate weakening
+-- Automatically applies `Derives.weakening` and tries to close the subset goal
+syntax "derive_weaken " term : tactic
+
+macro_rules
+  | `(tactic| derive_weaken $thm) => `(tactic| apply Derives.weakening $thm; repeat (apply List.subset_cons <|> exact List.Subset.refl _))
+
+-- Tactic to automate Reductio ad Absurdum (RAA)
+syntax "derive_raa" : tactic
+
+macro_rules
+  | `(tactic| derive_raa) => `(tactic| apply Derives.raa)
